cequiv/approx_star_swap.v
@@ -519,6 +519,168 @@ Proof.
 Qed.
 Hint Resolve implies_alpha_eq_bterm_mk_swap_cs2 : slow.
 
+Lemma flat_map_trivial :
+  forall {T} (l : list T),
+    flat_map (fun x => [x]) l = l.
+Proof.
+  induction l; introv; simpl; auto; try congruence.
+Qed.
+Hint Rewrite @flat_map_trivial : slow.
+
+Lemma alpha_eq_change_bvars_alpha {o} :
+  forall l (t : @NTerm o),
+    alpha_eq (change_bvars_alpha l t) t.
+Proof.
+  introv.
+  pose proof (change_bvars_alpha_spec t l) as q; simpl in *; repnd; eauto 3 with slow.
+Qed.
+Hint Resolve alpha_eq_change_bvars_alpha : slow.
+
+Lemma cswap_sub_disj {o} :
+  forall a b l k j,
+    disjoint j l
+    -> disjoint j k
+    -> @cswap_sub o (mk_swapping l k) (sw_sub a b j) = sw_sub a b j.
+Proof.
+  introv disja disjb.
+  unfold cswap_sub, sw_sub; rewrite map_map; unfold compose.
+  apply eq_maps; introv i; simpl.
+  applydup disja in i.
+  applydup disjb in i.
+  rewrite swapvar_not_in; tcsp.
+Qed.
+
+Hint Rewrite @osize_cswap : slow.
+
+Lemma implies_alpha_eq_lsubst_aux_sw_sub {o} :
+  forall a b (t u : @NTerm o) l,
+    alpha_eq t u
+    -> alpha_eq (lsubst_aux t (sw_sub a b l)) (lsubst_aux u (sw_sub a b l)).
+Proof.
+  nterm_ind1s t as [v|op bs ind] Case; introv aeq.
+  { inversion aeq; subst; simpl in *; tcsp. }
+  apply alpha_eq_oterm_implies_combine2 in aeq; exrepnd; subst; simpl in *.
+  unfold alpha_eq_bterms in *; repnd.
+
+  apply alpha_eq_oterm_combine; autorewrite with slow; dands; auto.
+  introv i.
+  rewrite <- map_combine in i.
+  apply in_map_iff in i; exrepnd; ginv.
+  destruct a1, a0; simpl in *.
+  applydup aeq0 in i1.
+
+  apply alphaeqbt_eq in i0.
+  apply alphaeqbt_eq; apply alphaeqbt_all; introv.
+  rw @alphaeqbt_all in i0; pose proof (i0 (l ++ l2)) as i0.
+  inversion i0 as [? ? ? ? ? disj lena lenb norep aeq']; subst; clear i0.
+  apply (aeqbt _ vs); auto.
+
+  { allrw disjoint_app_r; repnd; dands; auto;
+      apply disjoint_allvars_lsubst_aux; auto; autorewrite with slow;
+        rw flat_map_map; unfold compose; simpl; autorewrite with slow; eauto 3 with slow. }
+
+  assert (disjoint vs l0) as disj0.
+  { allrw disjoint_app_r; repnd; auto. }
+
+  assert (disjoint vs l1) as disj1.
+  { allrw disjoint_app_r; repnd; auto. }
+
+  assert (disjoint vs l) as disj2.
+  { allrw disjoint_app_r; repnd; auto. }
+
+  assert (disjoint vs (free_vars n)) as disj3.
+  { allrw disjoint_app_r; repnd; auto; introv i j.
+    apply free_vars_subset_allvars in j; apply lenb3 in j; tcsp. }
+
+  assert (disjoint vs (free_vars n0)) as disj4.
+  { allrw disjoint_app_r; repnd; auto; introv i j.
+    apply free_vars_subset_allvars in j; apply lenb in j; tcsp. }
+
+  repeat (rewrite lsubst_aux_cswap_cswap; auto; eauto 2 with slow).
+  autorewrite with slow.
+  apply alphaeq_vs_implies_alphaeq in aeq'; apply alphaeq_eq in aeq'.
+  apply alphaeq_implies_alphaeq_vs; apply alphaeq_eq.
+  repeat (rewrite cswap_sub_disj; eauto 3 with slow).
+
+  assert (subset (remove_nvars l0 l) l) as ssa by (introv i; apply in_remove_nvars in i; tcsp).
+  assert (subset (remove_nvars l1 l) l) as ssb by (introv i; apply in_remove_nvars in i; tcsp).
+  assert (subset (free_vars (cswap (mk_swapping l0 vs) n)) (remove_nvars l0 (free_vars n) ++ vs)) as ssc.
+  { introv i; rewrite free_vars_cswap in i; auto; eauto 2 with slow.
+    apply in_swapbvars in i; exrepnd; subst.
+    apply in_app_iff.
+    destruct (in_deq _ deq_nvar v' l0) as [d|d].
+    { right; apply swapvar_in; auto; eauto 2 with slow.
+      introv xx; apply disj3 in xx; tcsp. }
+    { rewrite swapvar_not_in; tcsp; try (complete (introv xx; apply disj3 in xx; tcsp)).
+      left; apply in_remove_nvars; tcsp. } }
+  assert (subset (free_vars (cswap (mk_swapping l1 vs) n0)) (remove_nvars l1 (free_vars n0) ++ vs)) as ssd.
+  { introv i; rewrite free_vars_cswap in i; auto; eauto 2 with slow.
+    apply in_swapbvars in i; exrepnd; subst.
+    apply in_app_iff.
+    destruct (in_deq _ deq_nvar v' l1) as [d|d].
+    { right; apply swapvar_in; auto; eauto 2 with slow.
+      introv xx; apply disj4 in xx; tcsp. }
+    { rewrite swapvar_not_in; tcsp; try (complete (introv xx; apply disj4 in xx; tcsp)).
+      left; apply in_remove_nvars; tcsp. } }
+
+  erewrite (implies_eq_lsubst_aux_sw_sub _ _ _ (remove_nvars l0 l)); eauto;
+    [|introv i j; apply ssc in j; apply in_remove_nvars; apply in_app_iff in j; dands; auto;
+      allrw in_remove_nvars; repndors; repnd; tcsp; apply disj0 in j; tcsp].
+
+  erewrite (implies_eq_lsubst_aux_sw_sub _ _ _ (remove_nvars l1 l)); eauto;
+    [|introv i j; apply ssd in j; apply in_remove_nvars; apply in_app_iff in j; dands; auto;
+      allrw in_remove_nvars; repndors; repnd; tcsp; apply disj1 in j; tcsp].
+
+  apply in_combine_left_eauto in i1.
+  eapply ind; eauto; autorewrite with slow; eauto 3 with slow.
+Qed.
+Hint Resolve implies_alpha_eq_lsubst_aux_sw_sub : slow.
+
+Lemma lsubst_sw_sub_alpha_eq_aux {o} :
+  forall (t : @NTerm o) a b l,
+    alpha_eq (lsubst t (sw_sub a b l)) (lsubst_aux t (sw_sub a b l)).
+Proof.
+  introv; unfold lsubst; autorewrite with slow.
+  rewrite flat_map_map; unfold compose; simpl; autorewrite with slow; boolvar; eauto 3 with slow.
+Qed.
+Hint Resolve lsubst_sw_sub_alpha_eq_aux : slow.
+
+Lemma implies_approx_star_push_swap_cs_sub_term {o} :
+  forall lib a b l (c d : @NTerm o),
+    approx_star lib c d
+    -> approx_star lib (push_swap_cs_sub_term a b l c) (push_swap_cs_sub_term a b l d).
+Proof.
+  introv apra.
+  unfold push_swap_cs_sub_term.
+  apply (lsubst_approx_star_congr3 _ _ _ (sw_sub a b l)) in apra; eauto 3 with slow.
+Qed.
+Hint Resolve implies_approx_star_push_swap_cs_sub_term : slow.
+
+Lemma implies_alpha_eq_bterm_mk_swap_cs2_push_swap_cs_sub_term {o} :
+  forall a b l1 l2 (t1 t2 : @NTerm o),
+    alpha_eq_bterm (bterm l1 t1) (bterm l2 t2)
+    -> alpha_eq_bterm
+         (bterm l1 (mk_swap_cs2 a b (push_swap_cs_sub_term a b l1 t1)))
+         (bterm l2 (mk_swap_cs2 a b (push_swap_cs_sub_term a b l2 t2))).
+Proof.
+  introv aeq.
+  inversion aeq as [? ? ? ? ? disj lena lenb norep aeq']; subst; clear aeq.
+  econstructor; try exact lenb; auto.
+
+  { unfold all_vars in *; simpl in *; autorewrite with slow; tcsp. }
+
+  allrw disjoint_app_r; repnd.
+  repeat (rewrite lsubst_lsubst_aux; simpl; autorewrite with slow;
+          [|rewrite flat_map_free_var_vars_range; auto; eauto 2 with slow; try omega];[]).
+  apply implies_alpha_eq_mk_swap_cs2.
+  unfold push_swap_cs_sub_term.
+
+  repeat (rewrite lsubst_aux_sw_sub_var_ren; auto; try omega;[]).
+  repeat (rewrite <- lsubst_push_swap_cs_sub_term_var_ren_eq2; auto; allrw disjoint_app_r; tcsp;[]).
+  apply implies_alpha_eq_lsubst_aux_sw_sub; auto.
+Qed.
+Hint Resolve implies_alpha_eq_bterm_mk_swap_cs2_push_swap_cs_sub_term : slow.
+
 Lemma approx_star_bterm_push_swap_cs_bterm {o} :
   forall lib can n1 n2 (b1 b2 : @BTerm o),
     approx_star_bterm lib (Can can) b1 b2
@@ -535,8 +697,8 @@ Proof.
   destruct b2 as [l2 t2].
   simpl in *.
 
-  exists lv (mk_swap_cs2 n1 n2 nt1) (mk_swap_cs2 n1 n2 nt2).
-  dands; eauto 3 with slow.
+  exists lv (mk_swap_cs2 n1 n2 (push_swap_cs_sub_term n1 n2 lv nt1)) (mk_swap_cs2 n1 n2 (push_swap_cs_sub_term n1 n2 lv nt2)).
+  dands; eauto 3 with slow;[].
   repndors; exrepnd;[left|right]; ginv.
   dands; tcsp; try (complete(intro xx; inversion xx)); eauto 3 with slow.
 Qed.
